\section{Self-Practice A4}

\begin{problem}
    Evaluate $\sum_{r = 2}^n \bp{2^{-r} + 2nr + n^2}$, giving your answer in terms of $n$.
\end{problem}
\begin{solution}
    Splitting the sum, we get \[\sum_{r = 2}^n \bp{2^{-r} + 2nr + n^2} = \sum_{r = 2}^n \bp{\frac12}^r + 2n \sum_{r = 2}^n r + n^2 \sum_{r = 2}^n 1.\] Hence,
    \begin{align*}
        \sum_{r = 2}^n  \bp{2^{-r} + 2nr + n^2} &= \bp{\frac12}^2 \bp{\frac{1 - (1/2)^{n-1}}{1 - 1/2}} + 2n \bp{\frac{n(n+1)}{2} - 1} + n^2 \bp{n - 1}\\
        &= \bs{\frac12 - \bp{\frac12}^n} + n^2 \bp{n+1} - 2n + n^2 \bp{n-1}\\
        &= \frac12 - \bp{\frac12}^n + 2n \bp{n^2 - 1}.
    \end{align*}
\end{solution}

\begin{problem}
    A geometric sequence $\bc{a_n}$ has first term $a$ and common ratio $r$. The sequence of numbers $\bc{b_n}$ satisfy the relation $b_n = \ln{a_n}$ for $n \in \ZZ^+$.

    \begin{enumerate}
        \item Show that $\bc{b_n}$ is an arithmetic sequence and determine the value of the common difference in terms of $r$.
        \item Find an expression for $\sum_{n = 1}^{N+1} b_n$ in terms of $a$, $a_{N+1}$ and $N$.
        \item Hence, obtain an expression for $a_1 \times a_2 \times \dots \times a_{N+1}$ in terms of $a$, $a_{N+1}$ and $N$.
    \end{enumerate}
\end{problem}
\begin{solution}
    \begin{ppart}
        Note that $a_n = ar^{n-1}$. Hence, \[b_n = \ln a_n = \ln{ar^{n-1}} = \ln a + (n-1) \ln r.\] Hence, \[b_n - b_{n-1} = \bs{\ln a + n \ln r} - \bs{\ln a + (n-1) \ln r} = \ln r.\] Thus, $\bc{b_n}$ is an arithmetic progression with common difference $\ln r$.
    \end{ppart}
    \begin{ppart}
        Since $\bc{b_n}$ is in arithmetic progression, we have \[\sum_{n = 1}^{N+1} b_n = \frac{N+1}{2} \bp{b_1 + b_{N+1}} = \frac{N+1}{2} \bp{\ln a_1 + \ln a_{N+1}} = \frac{N+1}{2} \ln{a a_{N+1}}.\]
    \end{ppart}
    \begin{ppart}
        Since $b_n = \ln a_n$, we can write the sum as \[\sum_{n = 1}^{N+1} b_n = \sum_{n = 1}^{N+1} \ln a_n = \ln \prod_{n = 1}^{N+1} a_n.\] Equating this with the above result yields \[\prod_{n = 1}^{N+1} a_n = \bp{a a_{N+1}}^{(N+1)/2}.\]
    \end{ppart}
\end{solution}

\clearpage
\begin{problem}
    It is given that $\sum_{r = 1}^n r^2 = \frac16 n(n+1)(2n+1)$.
    \begin{enumerate}
        \item Show that $\sum_{r = 1}^n (2r-7)(r+1) = \frac16 n\bp{4n^2 - 9n - 55}$.
        \item Find $\sum_{r = 1}^n 3^{-r}$ in terms of $n$, and find the least value of $n$ such that \[\sum_{r = 1}^n (2r-7)(r + 1) > \sum_{r = 1}^n 3^{-r}.\]
        \item Express $\sum_{r = n + 1}^{2n} (2r-7)(r+1)$ in terms of $n$.
        \item Hence, or otherwise, find the value of \[43\times26 + 45\times27 + 47\times28 + \dots +87\times48 + 89\times49.\]
    \end{enumerate}
\end{problem}
\begin{solution}
    \begin{ppart}
        Note that $(2r-7)(r+1) = 2r^2 -5r -7$. Hence,
        \begin{align*}
            \sum_{r = 1}^n (2r-7)(r+1) &= \sum_{r = 1}^n \bp{2r^2 - 5r - 7}\\
            &= 2\bp{\frac{n(n+1)(2n+1)}6} - 5\bp{\frac{n(n+1)}2} - 7n\\
            &= \frac{n\bp{4n^2 - 9n - 55}}6.
        \end{align*}
    \end{ppart}
    \begin{ppart}
        \[\sum_{r = 1}^n 3^{-r} = \sum_{r = 1}^n \bp{\frac13}^r = \bp{\frac13} \bp{\frac{1 - (1/3)^{n-1}}{1 - 1/3}} = \frac12 \bp{1 - \frac1{3^n}}.\] The inequality hence becomes \[\frac{n\bp{4n^2 - 9n - 55}}6 > \frac12 \bp{1 - \frac1{3^n}}.\] Using G.C., $n \geq 5.019$. Since $n$ is an integer, the least $n$ that satisfies the inequality is 6.
    \end{ppart}
    \begin{ppart}
        We have
        \begin{align*}
            \sum_{r = n + 1}^{2n} (2r-7)(r+1) &= \sum_{r = 1}^{2n} (2r-7)(r+1) - \sum_{r = 1}^{n} (2r-7)(r+1)\\
            &= \frac{2n\bs{4(2n)^2 - 9(2n) - 55}}6 - \frac{n\bp{4n^2 - 9n - 55}}6\\
            &= \frac{n\bp{28n^2 - 27n - 55}}6.
        \end{align*}
    \end{ppart}
    \begin{ppart}
        We have
        \begin{gather*}
            43\times26 + 45\times27 + 47\times28 + \dots +87\times48 + 89\times49 = \sum_{r = 24 + 1}^{2(24)} (2r-7)(r+1)\\
            = \frac{(24)\bs{28(24)^2 - 27(24) - 55}}6 = 61700.
        \end{gather*}
    \end{ppart}
\end{solution}

\clearpage
\begin{problem}
    It is given that $\sum_{r = 1}^n \frac{2r+1}{r(r+1)(r+2)} = \frac{n(5n+7)}{4(n+1)(n+2)}$.
    \begin{enumerate}
        \item Show that the series $\sum_{r = 1}^\infty \frac{2r+1}{r(r+1)(r+2)}$ converges and write down its sum to infinity.
        \item Find $\sum_{r = 0}^{n-2} \frac{2r+5}{(r+2)(r+3)(r+4)}$.
    \end{enumerate}
\end{problem}
\begin{solution}
    \begin{ppart}
        Clearly, \[\sum_{r = 1}^\infty \frac{2r+1}{r(r+1)(r+2)} = \lim_{n \to \infty} \frac{n(5n+7)}{4(n+1)(n+2)} = \lim_{n \to \infty} \frac{5 + \frac7n}{4 \bp{1 + \frac1n} \bp{1 + \frac2n}} = \frac54.\] Thus, the series converges and its sum to infinity is $5/4$.
    \end{ppart}
    \begin{ppart}
        Reindexing $r \mapsto r - 2$,
        \begin{gather*}
            \sum_{r = 0}^{n-2} \frac{2r+5}{(r+2)(r+3)(r+4)} = \sum_{r = 2}^n \frac{2r+1}{r(r+1)(r+2)} \\
            = \sum_{r = 1}^n \frac{2r+1}{r(r+1)(r+2)} - \frac{2(1) + 1}{1 (1 + 1) (1 + 2)} = \frac{n(5n+7)}{4(n+1)(n+2)} - \frac12.
        \end{gather*}
    \end{ppart}
\end{solution}