\section{Self-Practice A10.3}

\begin{problem}
    Express $\frac{\cot \t + \i}{\cot \t - \i}$ in the exponential form. Hence, show that one of the roots of the equation \[z^4 = \frac{\sqrt3 + \i}{\sqrt3 - \i}\] is $\e^{\i \pi/12}$, and find three more roots in the exponential form.
\end{problem}

\begin{problem}
    Find the cube roots of the complex number $1 + \i \sqrt3$. Give your answers exactly, in the form $r\e^{\i \t}$. Hence, solve the equation $z^6 - 2z^3 + 4 = 0$. Give your answers exactly, in the form $r\e^{\i \t}$.
\end{problem}

\begin{problem}
    Express $8\bp{\sqrt3 - \i}$ in the form $r\bp{\cos \t + \i \sin \t}$, where $r > 0$ and $-\pi \leq \t \leq \pi$, giving $\t$ in terms of $\pi$. Hence, obtain the roots of the equation $z^4 = 8\bp{\sqrt3 - \i}$ in the same form.
\end{problem}

\begin{problem}
    Write down, in any form, the five complex numbers which satisfy the equation $z^5 - 1 = 0$. Hence, show that the five complex numbers which satisfy the equation \[\bp{\frac{2w + 1}{w}}^5 = 1\] are \[\frac{-2 + \cos{\frac25 \pi k} - \i \sin{\frac25 \pi k}}{5 - 4 \cos{\frac25 \pi k}},\] where $k = 0, 1, 2, 3, 4$.
\end{problem}

\begin{problem}
    \begin{enumerate}
        \item Show that, for all complex numbers $z$ and all real numbers $\a$, \[\bp{z - \e^{\i \a}} \bp{z - \e^{-\i \a}} = z^2 - 2z\cos \a + 1.\]
        \item Write down, in any form, the seven complex numbers which satisfy the equation $z^7 - 1 = 0$.
        \item Hence, show that, for all complex numbers $z$, \[z^7 - 1 = (z-1)\bs{z^2 - 2z\cos \frac{2\pi}7 + 1}\bs{z^2 - 2z\cos \frac{4\pi}7 + 1}\bs{z^2 - 2z\cos \frac{6\pi}7 + 1}.\]
    \end{enumerate}
\end{problem}

\begin{problem}
    Use De Moivre's theorem to show that \[\cos 6\t = 32 \cos^6 \t - 48 \cos^4 \t + 18\cos^2 \t - 1.\] Deduce that, for all $\t$, \[0 \leq \cos^6 \t - \frac32 \cos^4 \t + \frac9{16} \cos^2 \t \leq \frac1{16}.\]
\end{problem}

\begin{problem}
    Show that for $z \neq -1$, \[z - z^2 + z^3 - \dots + z^7 = \frac{z + z^8}{1 + z}.\] Hence, by substituting $z = \e^{\i \t}$, show that \[\sum_{k=1}^7 (-1)^{k-1} \sin k\t = \frac{\sin 4\t \cos \frac72 \t}{\cos \frac12 \t},\] where $\t$ is not an odd multiple of $\pi$.
\end{problem}