\section{Tutorial B4}

\begin{problem}
    Evaluate the following limits.

    \begin{enumerate}
        \item $\lim\limits_{x \to 5} (6x + 7)$
        \item $\lim\limits_{x \to 1} \frac{x^3-1}{1-x}$
        \item $\lim\limits_{x \to \infty} \frac{3x}{2x^2-5}$
    \end{enumerate}
\end{problem}
\begin{solution}
    \begin{ppart}
        \[\lim_{x \to 5} (6x + 7) = 6(5) + 7 = 37.\]
    \end{ppart}
    \begin{ppart}
        \[\lim_{x \to 1} \frac{x^3-1}{1-x} = \lim_{x \to 1} \frac{(x-1)\bp{x^2 + x + 1}}{1-x} = \lim_{x \to 1} -\bp{x^2 + x + 1} = -(1^2 + 1 + 1) = -3.\]
    \end{ppart}
    \begin{ppart}
        \[\lim_{x \to \infty} \frac{3x}{2x^2-5} = \lim_{x \to \infty} \frac{3}{2x-5/x}.\] Note that as $x \to \infty$, $2x - \frac5{x} \to \infty$. Hence, $\lim\limits_{x \to \infty} \frac{1}{2x-5/x} = 0$.
    \end{ppart}
\end{solution}

\begin{problem}
    Differentiate the following with respect to $x$ from first principles.
        
    \begin{enumerate}
        \item $3x+4$
        \item $x^3$
    \end{enumerate}
\end{problem}
\begin{solution}
    \begin{ppart}
        \[\der{}{x} (3x+4) = \lim_{h \to 0}\frac{[3(x+h) + 4] - [3x + 4]}{h} = \lim_{h \to 0}\frac{3h}{h} = \lim_{h \to 0} 3 = 3.\]
    \end{ppart}
    \begin{ppart}
        \[\der{}{x} x^3 = \lim_{h \to 0} \frac{(x+h)^3 - x^3}{h} = \lim_{h \to 0} \frac{3hx^2 + 3h^2x + h^3}{h} = \lim_{h \to 0} \bp{3x^2 + 3hx + h^2} = 3x^2.\]
    \end{ppart}
\end{solution}

\clearpage
\begin{problem}
    Differentiate each of the following with respect to $x$, simplifying your answer.

    \begin{enumerate}
        \item $\bp{x^2 + 4}^2\bp{2x^3 -1}$
        \item $\frac{x^2}{\sqrt{4-x^2}}$
        \item $\sqrt{1+\sqrt x}$
        \item $\bp{\frac{x^3-1}{2x^3+1}}^4$
    \end{enumerate}
\end{problem}
\begin{solution}
    \begin{ppart}
        \begin{gather*}
            \der{}{x} \bp{x^2 + 4}^2\bp{2x^3 -1} = \bp{2x^3 - 1} \bs{4x \bp{x^2 + 4}} + \bp{x^2 + 4}^2\bp{6x^2}\\
            = 2x\bp{x^2 + 4}\bs{2\bp{2x^3 - 1} + 3x\bp{x^2 + 4}} = 2x\bp{x^2 + 4}\bp{7x^3 + 12x - 2}.
        \end{gather*}
    \end{ppart}
    \begin{ppart}
        \[\der{}{x} \frac{x^2}{\sqrt{4-x^2}} = \frac{\sqrt{4-x^2} \bp{2x} - x^2 \bp{\frac{-2x}{2\sqrt{4-x^2}}}}{4-x^2} = \frac{2x\bp{4-x^2} + x^3}{(4-x^2)^{3/2}} = \frac{x \bp{8-x^2}}{(4-x^2)^{3/2}}.\]
    \end{ppart}
    \begin{ppart}
        \[\der{}{x} \sqrt{1+\sqrt x} = \frac1{2\sqrt{1+\sqrt x}} \cdot \frac1{2\sqrt x} = \frac1{4\sqrt{x(1+\sqrt x)}}.\]
    \end{ppart}
    \begin{ppart}
        Note that \[\frac{x^3-1}{2x^3 + 1} = \frac12 \bp{\frac{2x^3 - 2}{2x^3 + 1}} = \frac12\bp{1 - \frac{3}{2x^3 + 1}} = \frac12 - \frac32 \bp{\frac{1}{2x^3 + 1}}.\] Hence, \[\der{}{x} \frac{x^3-1}{2x^3 + 1} = \der{}{x} \bs{\frac12 - \frac32 \bp{\frac{1}{2x^3 + 1}}} = -\frac32\bs{\frac{-6x^2}{\bp{2x^3 + 1}^2}} = \frac{9x^2}{\bp{2x^3 +1}^2}.\] Thus, \[\der{}{x} \bp{\frac{x^3-1}{2x^3+1}}^4 = 4\bp{\frac{x^3-1}{2x^3+1}}^3 \frac{9x^2}{\bp{2x^3 +1}^2} = \frac{36x^2\bp{x^3-1}^3}{\bp{2x^3+1}^5}.\]
    \end{ppart}
\end{solution}

\begin{problem}
    Using a graphing calculator, find the derivative of $\frac{\e^{2x}}{x^2+1}$ when $x = 1.5$.
\end{problem}
\begin{solution}
    \[\evalder{\der{}{x} \bp{\frac{\e^{2x}}{x^2+1}}}{x = 1.5} = 6.66.\]
\end{solution}

\begin{problem}
    Find the derivative with respect to $x$ of
        
    \begin{enumerate}
        \item $\cos x\deg$
        \item $\cot{1-2x^2}$
        \item $\tan^3 (5x)$
        \item $\frac{\sec x}{1 + \tan x}$
    \end{enumerate}
\end{problem}
\begin{solution}
    \begin{ppart}
        \[\der{}{x} \cos x\deg = \der{}{x} \cos{\frac{\pi}{180} x} = -\frac{\pi}{180} \sin{\frac{\pi}{180} x}.\]
    \end{ppart}
    \begin{ppart}
        \[\der{}{x} \cot{1-2x^2} = 4x\csc{1-2x^2}.\]
    \end{ppart}
    \begin{ppart}
        \[\der{}{x} \tan^3 (5x) = 15\tan^2(5x)\sec^2(5x).\]
    \end{ppart}
    \begin{ppart}
        Note that \[\frac{\sec x}{1 + \tan x} = \frac{1}{\sin x + \cos x} = \frac1{\sqrt2 \sin{x + \pi/4}} = \frac1{\sqrt2} \csc{x + \frac\pi4}.\] Hence, \[\der{}{x} \frac{\sec x}{1 + \tan x} = \der{}{x} \frac1{\sqrt2} \csc{x - \frac\pi4} = -\frac1{\sqrt2} \csc{x + \frac\pi4} \cot{x + \frac\pi4}.\]
    \end{ppart}
\end{solution}

\begin{problem}
    Find the derivative with respect to $x$ of

    \begin{enumerate}
        \item $y = \e^{1 + \sin 3x}$
        \item $y = x^2 \e^\frac1{x}$
        \item $y = \ln{\frac{1-x}{\sqrt{1+x^2}}}$
        \item $y = \frac{\ln{2x}}x$
        \item $y = \log_2 (3x^4 - \e^x)$
        \item $y = 3^{\ln \sin x}$
        \item $y = a^{2\log_a x}$
        \item $y = \sqrt[3]{\frac{\e^x (x+1)}{x^2 +1}}, \, x > 0$
    \end{enumerate}
\end{problem}
\begin{solution}
    \begin{ppart}
        \[\der{y}{x} =  \der{}{x} \e^{1 + \sin 3x} = 3 \e^{1 + \sin 3x} \cos{3x}.\]
    \end{ppart}
    \begin{ppart}
        \[\der{y}{x} = \der{}{x} x^2 \e^{1/x} = -x^2 \bp{-\frac{\e^{1/x}}{x^2}} + \e^{1/x}(2x) = \e^{1/x}(2x-1).\]
    \end{ppart}
    \begin{ppart}
        Note that \[y = \ln{\frac{1-x}{\sqrt{1 + x^2}}} = \ln{1-x} - \frac12 \ln{1 + x^2}.\] Hence, \[\der{y}{x} = \der{}{x} \bs{\ln{1-x} - \frac12 \ln{1 + x^2}} = -\frac1{1-x} - \frac{x}{1 + x^2} = -\frac{1 + x}{(1-x)\bp{1 + x^2}}.\]
    \end{ppart}
    \begin{ppart}
        \[\der{y}{x} = \der{}{x} \frac{\ln{2x}}x = \frac{x \bp{\frac1x} - \ln{2x}(1)}{x^2} = \frac{1 - \ln{2x}}{x^2}.\]
    \end{ppart}
    \begin{ppart}
        Note that \[y = {\log_2} {\bp{3x^4 - \e^x}} \implies 2^y = 3x^4 - \e^x.\] Implicitly differentiating with respect to $x$, \[2^y \ln 2 \cdot \der{y}{x} = 12x^3 - \e^x \implies \der{y}{x} = \frac{12x^3 - \e^x}{2^y \ln 2} =  \frac{12x^3 - \e^x}{\bp{3x^4 - \e^x}\ln 2}.\]
    \end{ppart}
    \begin{ppart}
        Note that \[y = 3^{\ln \sin x} \implies \log_3 y = \frac{\ln y}{\ln 3} = \ln \sin x \implies \ln y = \ln 3 \ln \sin x.\] Implicitly differentiating with respect to $x$, \[\frac1y \cdot \der{y}{x} = \ln 3 \bp{\frac{\cos x}{\sin x}} = \ln 3 \cdot \cot x \implies \der{y}{x} = \ln 3 \cdot y \cot x = \ln 3 \cdot \cot{x} \cdot 3^{\ln \sin x}.\]
    \end{ppart}
    \begin{ppart}
        Observe that \[y = a^{2\log_a x} = a^{\log_a x^2} = x^2 \implies \der{y}{x} = \der{}{x} x^2 = 2x.\]
    \end{ppart}
    \begin{ppart}
        Note that \[y = \sqrt[3]{\frac{\e^x (x+1)}{x^2 +1}} \implies \bp{x^2 + 1} y^3 = \e^x (x + 1).\] Implicitly differentiating with respect to $x$, \[\bp{x^2 + 1}\bp{3y^2 \cdot \der{y}{x}} + y^3 \bp{2x} = \e^x + (x+1)\e^x \implies \der{y}{x} = \frac{\e^x (x+2) - 2xy^3}{3\bp{x^2 + 1}y^2}.\] Now observe that \[\frac{\e^x (x+2)}{3\bp{x^2 + 1}y^2} = \frac{\e^x (x+1)(x+2)}{3\bp{x^2 + 1}(x+1)y^2} = \frac{y^3 (x+2)}{3(x+1)y^2} = y\bp{\frac{x+2}{3(x+1)}}.\] Thus, \[\der{y}{x} = y\bp{\frac{x+2}{3(x+1)}} - y\bp{\frac{2x}{3\bp{x^2 + 1}}} = \frac13 \sqrt[3]{\frac{\e^x (x+1)}{x^2 +1}} \bp{\frac{x+2}{x+1} - \frac{2x}{x^2 + 1}}.\]
    \end{ppart}
\end{solution}

\clearpage
\begin{problem}
    Find the derivative with respect to $x$ of

    \begin{enumerate}
        \item $\arccos{\frac{x}{10}}$
        \item $\arctan{\frac1{1-x}}$
        \item $\arcsin{\tan x}$
    \end{enumerate}
\end{problem}
\begin{solution}
    \begin{ppart}
        \[\der{}{x} \arccos \frac{x}{10} = -\frac1{10\sqrt{1-\bp{\frac{x}{10}}^2}} = -\frac{1}{\sqrt{100 - x^2}}.\]
    \end{ppart}
    \begin{ppart}
        \[\der{}{x} \arctan{\frac1{1-x}} = \frac{1}{1 + \bp{\frac1{1-x}}^2} \bp{\frac1{(1-x)^2}} = \frac1{(1-x)^2+1}.\]
    \end{ppart}
    \begin{ppart}
        \[\der{}{x} \arcsin (\tan x) = \frac{\sec^2x}{1-\tan^2 x}.\]
    \end{ppart}
\end{solution}

\begin{problem}
    Find an expression for $\derx{y}{x}$ in terms of $x$ and $y$.
        
    \begin{enumerate}
        \item $(y-x)^2 = 2a(y+x)$, where $a$ is a constant
        \item $y^2 = \e^{2x}y + x\e^x$
        \item $y = x^y$
        \item $\sin x \cos y = \frac12$
    \end{enumerate}
\end{problem}
\begin{solution}
    \begin{ppart}
        Implicitly differentiating with respect to $x$, \[(y-x)\bp{\der{y}{x} - 1} = a\bp{\der{y}{x} + 1} \implies \der{y}{x} = \frac{a + y - x}{y - x - a}.\]
    \end{ppart}
    \begin{ppart}
        Implicitly differential with respect to $x$, \[2y \cdot \der{y}{x} = \bp{\e^{2x} \der{y}{x} + 2ye^{2x}} + \bp{x\e^x + \e^x} \implies \der{y}{x} = \frac{\e^x \bp{2y\e^x + x + 1}}{2y - \e^{2x}}.\]
    \end{ppart}
    \begin{ppart}
        Note that \[y = x^y \implies \ln y = y \ln x.\] Implicitly differentiating with respect to $x$, \[\frac1y \cdot \der{y}{x} = \frac{y}{x} + \ln x \cdot \der{y}{x} \implies \der{y}{x} = \frac{y/x}{1/y - \ln x} = \frac{y^2}{x - xy \ln x}.\]
    \end{ppart}
    \begin{ppart}
        Note that \[\sin x \cos y  = \frac12 \implies \cos y = \frac12 \csc x.\] Implicitly differentiating with respect to $x$, \[-\sin y \cdot \der{y}{x} = -\frac12 \csc x \cot x \implies \der{y}{x} = \frac{\csc x \cot x}{2\sin y}.\]
    \end{ppart}
\end{solution}

\begin{problem}
    It is given that $x$ and $y$ satisfy the equation \[\arctan x + \arctan y  + \arctan{xy} = \frac7{12} \pi.\]

    \begin{enumerate}
        \item Find the exact value of $y$ when $x = 1$.
        \item Express $\der{}{x} \arctan{xy}$ in terms of $x$, $y$ and $y'$.
        \item Show that, when $x = 1$, $y' = -\frac13 - \frac1{2\sqrt3}$.
    \end{enumerate}
\end{problem}
\begin{solution}
    \begin{ppart}
        Substituting $x = 1$ into the given equation, \[\frac14 \pi + 2\arctan y = \frac{7\pi}{12} \implies \arctan y = \frac\pi6 \implies y = \frac1{\sqrt3}.\]
    \end{ppart}
    \begin{ppart}
        \[\der{}{x} \arctan{xy} = \frac{xy' + y}{1+(xy)^2}.\]
    \end{ppart}
    \begin{ppart}
        Differentiating the given equation with respect to $x$, \[\frac{1}{1+x^2} + \frac{y'}{1+y^2} + \frac{xy' + y}{1+(xy)^2} = 0.\] Substituting $x=1$, \[\frac12 + \frac{3y'}4 + \frac34\bp{y' + \frac1{\sqrt3}} = 0 \implies y' = \frac23 \bp{-\frac3{4\sqrt3} - \frac12} = -\frac1{2\sqrt3} - \frac13.\]
    \end{ppart}
\end{solution}

\begin{problem}
    Find $\derx{y}{x}$ for

    \begin{enumerate}
        \item $x = \frac1{1+t^2}, \, y = \frac{t}{1+t^2}$
        \item $x = \frac12 (\e^t - \e^{-t}), \, y = \frac12 (\e^t + \e^{-t})$
        \item $x = a\sec\t, \, y = a\tan\t$
        \item $x = \e^{3\t}\cos{3\t}, \, y = \e^{3\t}\sin{3\t}$
    \end{enumerate}
\end{problem}
\begin{solution}
    \begin{ppart}
        Observe that $y = xt$. Hence, \[\der{y}{x} = x\bp{\der{t}{x}} + t = x \bp{\der{x}{t}}^{-1} + t = \frac1{1 + t^2} \bp{-\frac{2t}{\bp{1 + t^2}^2}}^{-1} + t = \frac{t^2-1}{2t}.\]
    \end{ppart}
    \begin{ppart}
        \[\der{y}{x} = \frac{\derx{y}{t}}{\derx{x}{t}} = \frac{\frac12 \bp{\e^t - \e^{-t}}}{\frac12 \bp{\e^t + \e^{-t}}} = \frac{\e^t - \e^{-t}}{\e^t + \e^{-t}}.\]
    \end{ppart}
    \begin{ppart}
        Recall that $\tan^2 \t + 1 = \sec^2 \t$. Hence, $y^2 + a^2 = x^2$. Implicitly differentiating with respect to $x$, we have \[2y\cdot\der{y}{x} = 2x \implies \der{y}{x} = \frac{x}{y} = \frac{a\sec \t}{a \tan \t} = \csc \t.\]
    \end{ppart}
    \begin{ppart}
        \[\der{y}{x} = \frac{\derx{y}{(3\t)}}{\derx{x}{(3\t)}} = \frac{\e^{3\t} \cos 3\t + \e^{3\t} \sin 3\t}{-\e^{3\t} \sin 3\t + \e^{3\t} \cos 3\t} = \frac{\cos 3\t + \sin 3\t}{\cos 3\t - \sin 3\t}.\]
    \end{ppart}
\end{solution}

\begin{problem}
    A curve is defined by the parametric equation \[x = 120t - 4t^2, \, y = 60t - 6t^2.\] Find the value of $\derx{y}{x}$ at each of the points where the curve cross the $x$-axis.
\end{problem}
\begin{solution}
    The curve crosses the $x$-axis when $y=0$: \[y = 60t-6t^2 = 6t(10 - t) = 0.\] Hence, $t = 0$ or $t = 10$. Now, consider the derivative with respect to $x$ of the curve. \[\der{y}{x} = \frac{\derx{y}{t}}{\derx{x}{t}} = \frac{60 - 12t}{120 - 8t}.\]

    \case{1}[$t =0$] \[\evalder{\der{y}{x}}{t = 0} = \frac{60 - 12(0)}{120 - 8(0)} = \frac12.\]

    \case{2}[$t=10$] \[\evalder{\der{y}{x}}{t = 10} = \frac{60 - 12(10)}{120 - 8(10)} = -\frac32.\]
\end{solution}

\begin{problem}
    A curve has parametric equations $x = 2t-\ln{2t}, \, y = t^2 - \ln t^2$, where $t > 0$. Find the value of $t$ at the point on the curve at which the gradient is 2.
\end{problem}
\begin{solution}
    \[\der{y}{x} = \frac{\derx{y}{t}}{\derx{x}{t}} = \frac{2t - 2/t}{2 - 1/t} = \frac{2t^2 - 2}{2t - 1}.\] Consider $\derx{y}{x} = 2$. \[\der{y}{x} = \frac{2t^2 - 2}{2t - 1} = 2 \implies \frac{t^2 - 1}{2t - 1} = 1 \implies t^2 - 1 = 2t - 1 \implies t^2 - 2t = t(t - 2) = 0.\] Hence, $t = 0$ or $t = 2$. Since $t > 0$, we reject $t = 0$. Thus, $t = 2$.
\end{solution}

\clearpage
\begin{problem}
    If $y = \ln{\sin^3 2x}$, find $\der{y}{x}$ and prove that $3\der[2]{y}{x} + \bp{\der{y}{x}}^2 + 36 = 0$.
\end{problem}
\begin{solution}
    \[\der{y}{x} = \frac{6\sin^2 2x \cos 2x}{\sin^3 2x} = 6\cot 2x.\] Hence, \[\der[2]{y}{x} = -12\csc^2 2x = -12 \bp{1 + \cot^2 2x} = -12 - \frac13 \bp{\der{y}{x}}^2.\] Thus, we clearly have \[3\der[2]{y}{x} + \bp{\der{y}{x}}^2 + 36 = 0.\]
\end{solution}

\begin{problem}
    Given that $y = \e^{\arcsin{2x}}$, show that $\bp{1-4x^2}\der[2]{y}{x} - 4x\der{y}{x} = 4y$. Differentiate this result further to obtain a differential equation for $\der[3]{y}{x}$.
\end{problem}
\begin{solution}
    Note that \[y = \e^{\arcsin{2x}} \implies \ln y = \arcsin{2x}.\] Implicitly differentiating with respect to $x$, \[\frac1y \cdot \der{y}{x} = \frac2{\sqrt{1 - 4x^2}} \implies \der{y}{x} = \frac{2y}{\sqrt{1 - 4x^2}}.\] Implicitly differentiating with respect to $x$ once again, \[\der[2]{y}{x} = \frac{\sqrt{1 - 4x^2} \bp{2 \cdot \der{y}{x}} - 2y \bp{\frac{-4x}{\sqrt{1 - 4x^2}}}}{1 - 4x^2}.\] Now observe that \[2\sqrt{1 - 4x^2} \cdot \der{y}{x} + 4x \bp{\frac{2y}{\sqrt{1 - 4x^2}}} = 4y + 4x \cdot \der{y}{x}.\] Hence, \[\bp{1 - 4x^2}\der[2]{y}{x} = 4y + 4x\cdot\der{y}{x} \implies \bp{1-4x^2}\der[2]{y}{x} - 4x \cdot \der{y}{x} = 4y.\] Implicitly differentiating with respect to $x$ once again, \[\bp{1 - 4x^2} \der[3]{y}{x} -8x \cdot \der[2]{y}{x} -4 \bp{x \cdot \der[2]{y}{x} + \der{y}{x}} = 4\cdot \der{y}{x}.\] Rearranging, \[\bp{1 - 4x^2} \der[3]{y}{x} -12x \cdot \der[2]{y}{x} - 8 \cdot\der{y}{x} = 0.\]
\end{solution}