\documentclass{echw}

\title{Tutorial B11\\Functions of Two Variables}
\author{Eytan Chong}
\date{2024-07-26}

\begin{document}
    \problem{}
        Find the natural domain of the function $f$ for the following:
        \begin{enumerate}
            \item $f(x, y) = \sqrt{1 - x^2 - y^2}$
            \item $f(x, y) = \ln{x^2 - y}$
            \item $f(x, y) = \arcsin{x + y}$
            \item $f(x, y) = \dfrac1{x^2 - y^2}$
        \end{enumerate}

    \solution
        \part
            Observe that the argument of the square root must be non-negative. Hence, $1 - x^2 - y^2 \geq 0 \implies x^2 + y^2 \leq 1$.

            \boxt{$\dom f = \{ (x, y) \in \R^2 : x^2 + y^2 \leq 1\}$}

        \part
            Observe that the argument of the natural log must be positive. Hence, $x^2 - y > 0 \implies y < x^2$.

            \boxt{$\dom f = \{(x, y) \in \R^2 : y < x^2\}$}

        \part
            Observe that the argument of $\arcsin$ must be within the range of $\sin$, i.e. between $-1$ and 1 inclusive. Hence, $-1 \leq x + y \leq 1$.

            \boxt{$\dom f = \{(x, y) \in \R^2 : -1 \leq x + y \leq 1\}$}
        
        \part
            Observe that the denominator must be non-zero. Hence, $x^2 - y^2 \neq 0 \implies y^2 \neq x^2 \implies y \neq x \lor y \neq -x$.

            \boxt{$\dom f = \{(x, y) \in \R^2 : y \neq x \lor y \neq -x\}$}

    \problem{}
        Identify the correct equations of the following surfaces in 3-D space.

        \begin{itemize}
            \item $z = \cos{x + y}$
            \item $z = x^2y + 1$
            \item $z = 3 - x + y$
            \item $z = -\dfrac1{\sqrt{x^2 + y^2}}$
        \end{itemize}

        \begin{enumerate}
            \item \begin{center}
                \begin{tikzpicture}[trim axis left, trim axis right]
                    \begin{axis}[
                        axis on top,
                        axis y line=middle,
                        axis x line=middle,
                        axis z line=middle,
                        xtick = \empty,
                        ytick = \empty,
                        ztick = \empty,
                        xlabel = {$x$},
                        ylabel = {$y$},
                        zlabel = {$z$},
                        zmax = 10,
                        zmin = -10,
                        legend cell align={left},
                        legend pos=outer north east,
                        ]
                        \addplot3[surf,shader=faceted interp, colormap/hot,opacity=0.7]{x^2 * y + 1};
                    \end{axis}
                \end{tikzpicture}
            \end{center}
            \item \begin{center}
                \begin{tikzpicture}[trim axis left, trim axis right]
                    \begin{axis}[
                        axis on top,
                        axis y line=middle,
                        axis x line=middle,
                        axis z line=middle,
                        xtick = \empty,
                        ytick = \empty,
                        ztick = \empty,
                        xlabel = {$x$},
                        ylabel = {$y$},
                        zlabel = {$z$},
                        samples=50,
                        legend cell align={left},
                        legend pos=outer north east,
                        ]
                        \addplot3[surf,shader=faceted interp, colormap/hot,opacity=0.7, ]{-1/(x^2 + y^2)};
                    \end{axis}
                \end{tikzpicture}
            \end{center}
            \item \begin{center}
                \begin{tikzpicture}[trim axis left, trim axis right]
                    \begin{axis}[
                        axis on top,
                        axis y line=middle,
                        axis x line=middle,
                        axis z line=middle,
                        xtick = \empty,
                        ytick = \empty,
                        ztick = \empty,
                        xlabel = {$x$},
                        ylabel = {$y$},
                        zlabel = {$z$},
                        legend cell align={left},
                        legend pos=outer north east,
                        ]
                        \addplot3[surf,shader=faceted interp, colormap/hot,opacity=0.7, ]{cos(\x r + \y r)};
                    \end{axis}
                \end{tikzpicture}
            \end{center}
            \item \begin{center}
                \begin{tikzpicture}[trim axis left, trim axis right]
                    \begin{axis}[
                        axis on top,
                        axis y line=middle,
                        axis x line=middle,
                        axis z line=middle,
                        xtick = \empty,
                        ytick = \empty,
                        ztick = \empty,
                        xlabel = {$x$},
                        ylabel = {$y$},
                        zlabel = {$z$},
                        legend cell align={left},
                        legend pos=outer north east,
                        ]
                        \addplot3[surf,shader=faceted interp, colormap/hot,opacity=0.7, ]{3 - x + y};
                    \end{axis}
                \end{tikzpicture}
            \end{center}
        \end{enumerate}
        
        \part
            \boxt{$z = x^2 y + 1$}

        \part
            \boxt{$z = -\dfrac1{\sqrt{x^2 + y^2}}$}

        \part
            \boxt{$z = \cos{x + y}$}

        \part
            \boxt{$z = 3 - x + y$}

    \problem{}
        Let $f(x, y) = x^2 - 2x^3 + 3xy$. Find an equation of the level curve that passes through the point
        \begin{enumerate}
            \item $(-1, 1)$
            \item $(2, -1)$
            \item $(1, 5)$
        \end{enumerate}

    \solution
        \part
            Note that $f(-1, 1) = 0$. Hence, the level curve is given by $\boxed{x^2 - 2x^3 + 3xy = 0}$.

        \part
            Note that $f(2, -1) = -18$. Hence, the level curve is given by $\boxed{x^2 - 2x^3 + 3xy = -18}$.

        \part
            Note that $f(1, 5) = 14$. Hence, the level curve is given by $\boxed{x^2 - 2x^3 + 3xy = 14}$.

    \problem{}
        If $V(x, y)$ is the voltage or potential at a point $(x, y)$ in the $xy$-plane, then the level curves of $V$ are called equipotential curves. Along such a curve, the voltage remains constant. Given that \[V(x, y) = \dfrac{8}{\sqrt{16 + x^2 + y^2}}\] find an equation of the equipotential curves at which
        \begin{enumerate}
            \item $V = 2.0$
            \item $V = 1.0$
            \item $V = 0.5$
        \end{enumerate}

    \solution
        Rearranging the given equation, we have \[x^2 + y^2 = \dfrac{64}{V^2} - 16.\]

        \part
            When $V = 2.0$, we have $x^2 + y^2 = \dfrac{64}{2.0^2} - 16 = 0$, whence $x = 0$ and $y = 0$.

            \boxt{$x = 0 \land y = 0$}

        \part
            When $V = 1.0$, we have $x^2 + y^2 = \dfrac{64}{1.0^2} - 16 = 48$.

            \boxt{$x^2 + y^2 = 48$}

        \part
            When $V = 0.5$, we have $x^2 + y^2 = \dfrac{64}{0.5^2} - 16 = 240$.

            \boxt{$x^2 + y^2 = 240$}

    \problem{}
        Given that $f(x, y) = x^4 \sin{xy^3}$, find $f_x(x, y)$, $f_y(x, y)$, $f_{xy}(x, y)$ and $f_{yx}(x, y)$.

    \solution
        Differentiating $f$ with respect to $x$,
        \boxt{$f_x(x, y) = 4x^3 \sin{xy^3} + x^4 y^3 \cos{xy^3}$}

        Differentiating $f$ with respect to $y$,
        \boxt{$f_y(x, y) = 3x^5y^2\cos{xy^3}$}

        Differentiating $f_x$ with respect to $y$, 
        \begin{align*}
            f_{xy}(x, y) &= 12x^4y^2\cos{xy^3} + x^4\bs{3y^2\cos{xy^3} - 3xy^5\sin{xy^3}}\\
            &= 15x^4y^2\cos{xy^3} - 3x^5y^5\sin{xy^3}
        \end{align*}

        \boxt{$f_{xy}(x, y) = 15x^4y^2\cos{xy^3} - 3x^5y^5\sin{xy^3}$}

        Differentiating $f_y$ with respect to $x$,
        \begin{align*}
            f_{yx}(x, y) &= 3y^2\bs{5x^4 \cos{xy^3} - x^5y^3\sin{xy^3}}\\
            &= 15x^4y^2 \cos{xy^3} - 3x^5y^5 \sin{xy^3}
        \end{align*}

        \boxt{$f_{yx}(x, y) = 15x^4y^2\cos{xy^3} - 3x^5y^5\sin{xy^3}$}

    \problem{}
        Given that $z = x^2y$, $x = t^2$, $y = t^3$, use the chain rule to find $\der{z}{t}$ in terms of $t$.

    \solution
        \begin{align*}
            \der{z}{t} &= \pder{z}{x} \cdot \der{x}{t} + \pder{z}{y} \cdot \der{y}{t}\\
            &= 2xy \cdot 2t + x^2 \cdot 3t^2\\
            &= 2t^2t^3 \cdot 2t + (t^2)^2 \cdot 3t^2\\
            &= 7t^6
        \end{align*}

        \boxt{$\der{z}{t} = 7t^6$}

    \problem{}
        Find the gradient of $f(x, y) = 3x^2y$ at the point $(1, 2)$ and use it to calculate the directional derivative of $f$ at $(1, 2)$ in the direction of the vector $\vec u = 3\vec i + 4\vec j$.

    \solution
        Note that $f_x(x, y) = 6xy$ and $f_y(x, y) = 3x^2$. Hence, $\nabla f$ at $(1, 2)$ is given by $\cvecii{12}{3}$. 
        
        \boxt{The derivative at $(1, 2)$ is $\cvecii{12}3$.}
        
        Observe that the directional derivative of $f$ in the direction of $\vec u$ at $(1, 2)$ is given by \[\nabla f \cdot \hat{\vec u} = \cvecii{12}3 \cdot \dfrac15 \cvecii34 = \dfrac{48}5\]

        \boxt{The instantaneous rate of change at $(1, 2)$ in the direction of $\vec u$ is $\dfrac{48}5$.}

    \problem{}
        Suppose that a point moves along the intersection of the sphere $x^2 + y^2 + z^2 = 1$ with the plane $x = \dfrac23$. Find the rate of $z$ with respect to $y$ when the point is at $\bp{\dfrac23, \dfrac13, \dfrac23}$.

    \solution
        Note that $x^2 + y^2 + z^2 = 1 \implies z = \pm \sqrt{1 - x^2 - y^2}$. Given that the object we want (the rate of change of $z$ with respect to $y$) will later be evaluated when $z = \dfrac23 > 0$, we consider only the positive branch. Let $f(x, y) = \sqrt{1 - x^2 - y^2}$. Then $f_y(x, y) = \dfrac{-y}{\sqrt{1 - x^2 - y^2}}$. Evaluating at the desired point, we get, $f_y\bp{\dfrac23, \dfrac13} = \dfrac{-1/3}{\sqrt{1 - (2/3)^2 - (1/3)^2}} = -\dfrac12$.

        \boxt{The rate of change of $z$ with respect to $y$ at $\bp{\dfrac23, \dfrac13, \dfrac23}$ is $-\dfrac12$.}

    \problem{}
        \begin{enumerate}
            \item The Cauchy-Riemann equations are such that $\pder{u}{x} = \pder{v}{y}$ and $\pder{u}{y} = -\pder{v}{x}$ for $u(x, y)$ and $v(x, y)$. Show that $u = e^x \cos y$, $v = e^x \sin y$ satisfy the Cauchy-Riemann equations.
            \item Show that the function $f(x, y) = e^x \sin y + e^y \cos x$ satisfies that Laplace equation, i.e. $\pder[2]{f}{x} + \pder[2]{f}{y} = 0$.
            \item If $u(x, y)$ and $v(x, y)$ satisfy the Cauchy-Riemann equations, state the conditions for both $u$ and $v$ to satisfy the Laplace equation.
        \end{enumerate}

    \solution
        \part
            Differentiating $u$ with respect to $x$, $\pder{u}{x} = e^x \cos y$. Differentiating $v$ with respect to $y$, $\pder{v}{y} = e^x \cos y$. Hence, $\pder{u}{x} = \pder{v}{y}$.

            Differentiating $u$ with respect to $y$, $\pder{u}{y} = -e^x \sin y$. Differentiating $v$ with respect to $x$, $\pder{v}{x} = e^x \sin y$. Hence, $\pder{u}{y} = -\pder{v}{x}$.
            
            Thus, $u$ and $v$ satisfy the Cauchy-Riemann equations.

        \part
            Differentiating $f$ twice with respect to $x$,
            \[
                \pder[2]{f}{x} = \pder{f}{x} (e^x \sin y - e^y \sin x) = e^x \sin y - e^y \cos x
            \]
            Differentiating $f$ twice with respect to $y$,
            \[
                \pder[2]{f}{y} = \pder{f}{y} (e^x \cos y + e^y \cos x) = -e^x \sin y + e^y \cos x
            \]
            Hence,
            \[
                \pder[2]{f}{x} + \pder[2]{f}{y} = (e^x \sin y - e^y \cos x) + (-e^x \sin y + e^y \cos x) = 0
            \]
            Thus, $f(x, y) = e^x \sin y + e^y \cos x$ satisfies the Laplace equation.

        \part
            Suppose $u(x, y)$ and $v(x, y)$ satisfy the Cauchy-Riemann equations. This gives
            \[\begin{cases}
                \begin{aligned}
                    u_x &= v_y\\
                    u_y &= -v_x
                \end{aligned}
            \end{cases}
            \]
            Differentiating with respect to $x$, we obtain
            \[\begin{cases}
                \begin{aligned}
                    u_{xx} &= v_{yx}\\
                    u_{yx} &= -v_{xx}
                \end{aligned}
            \end{cases}
            \]
            Differentiating with respect to $y$, we obtain
            \[\begin{cases}
                \begin{aligned}
                    u_{xy} &= v_{yy}\\
                    u_{yy} &= -v_{xy}
                \end{aligned}
            \end{cases}
            \]
            This gives
            \[\begin{cases}
                \begin{aligned}
                    u_{xx} + u_{yy} &= v_{yx} - v_{xy}\\
                    v_{xx} + v_{yy} &= -u_{yx} + u_{xy}\\
                \end{aligned}
            \end{cases}
            \]
            Hence, if $u$ and $v$ both satisfy the Laplace equation, we require 
            \[\begin{cases}
                \begin{aligned}
                    v_{yx} - v_{xy} &= 0\\
                    -u_{yx} + u_{xy} &= 0\\
                \end{aligned}
            \end{cases}
            \]
            which gives the conditions $u_{xy} = u_{yx}$ and $v_{xy} = v_{yx}$.

            \boxt{$u_{xy} = u_{yx}$, $v_{xy} = v_{yx}$}


    \problem{}
        Find the equation of the tangent plane to the surface $z = x^2 y$ at the point $(2, 1, 4)$. Hence, state the normal vector of the tangent plane.

    \solution
        Let $f(x, y) = x^2y$. Then $f_x(x, y) = 2xy$ and $f_y(x, y) = x^2$. Hence, the equation of the tangent plane at $(2, 1, 4)$ is given by 
        \begin{alignat*}{2}
            &&z &= 4 + f_x(2, 1)(x-2) + f_y(y - 1)\\
            && &= 4 + 4(x-2) + 4(y-1)\\
            && &= 4x + 4y - 8\\
            \implies&&4x + 4y - z &= 8
        \end{alignat*}

        \boxt{$4x + 4y - z = 8$, $\vec n = \cveciii44{-1}$}

    \problem{}
        The volume of a right-circular cone of radius $r$ cm and height $h$ cm is denoted by $V$. If $h$ increases from $10$ cm to $10.01$ cm and $r$ decreases from $12$ cm to $11.95$ cm, use a linear approximation to estimate the volume of the cone after the changes.

    \solution
        Let $V(r, h) = \dfrac13 \pi r^2 h$ be the volume of the cone. We have $V_r(r, h) = \dfrac23 \pi r h$ and $V_h(r, h) = \dfrac13 \pi r^2$. The equation of the tangent plane at $r = 12$ and $h = 10$ is given by
        \begin{align*}
            v &= V(12, 10) + V_r(12, 10)(r-12) + V_h(12, 10)(h-10)\\
            &= \dfrac13\pi(12^2)(10) + \dfrac23 \pi(12)(10)(r - 12) + \dfrac13 \pi (12^2) (h-10)\\
            &= 16\pi(5r + 3h - 60)
        \end{align*}
        Evaluating at $r = 11.95$ and $h = 10.01$, we have
        \[v = 16\pi\bs{5\cdot11.95 + 3\cdot10.01 - 60} = 476.48\pi\]
        \boxt{The volume of the cone after the changes is approximately $476.48\pi$ cm$^3$.}       

    \problem{}
        The radius of a right-circular cylinder is measured with an error of at most $2\%$, and the height is measured with an error of at most 4\%. Approximate the maximum possible percentage error in the volume of the cylinder calculated from these measurements.

    \solution
        Let the volume of the cylinder be $V = \pi r^2 h$.
        \begin{alignat*}{2}
            && \d V &= \pder{V}{r} \d r + \pder{f}{h} \d h\\
            && &= 2\pi rh \d  r + \pi r^2 \d h\\
            \implies&&\dfrac{\d V}{V} &= \dfrac{2\pi rh \d  r + \pi r^2 \d h}{\pi r^2 h}\\
            && &= 2 \dfrac{\d r}{r} + \dfrac{\d h}{h}
        \end{alignat*}
        Note that $\dfrac{\d V}{V}$ measures the percentage error of the volume $V$, while $\dfrac{\d r}{r}$ and $\dfrac{\d h}{h}$ measure the percentage error of the radius and height respectively. Hence, \[\max \dfrac{\d V}{V} = 2(2\%) + 4\% = 8\%\]

        \boxt{The maximum percentage error in the volume of the cylinder is 8\%.}

    \problem{}
        On a certain mountain, the elevation $z$ above a point $(x, y)$ in a horizontal $xy$-plane that lies at sea level is $z = 2000 - 2x^2 - 4y^2$ ft. The positive $x$-axis points east, and the positive $y$-axis points north. A climber is at the point $(-20, 5, 1100)$.

        \begin{enumerate}
            \item If the climber uses a compass reading to walk due northeast, will he ascend or descend? Find this rate.
            \item Find the direction where the climber should walk to travel a level path.
        \end{enumerate}

    \solution
        \part
            Let $f(x, y) = 2000 - 2x^2 - 4y^2$. Then $f_x(x, y) = -4x$ and $f_y(x, y) = -8y$. Hence, \[\nabla f = \cvecii{-4x}{-8y} = -4\cvecii{x}{2y}\]
            Note that the vector $\cvecii11$ points northeast.
            \[
                \nabla f \cdot \widehat{\cvecii11} = -4\cvecii{x}{2y} \cdot \dfrac{\sqrt2}{2} \cvecii11 = -2\sqrt2 \bp{x + 2y}
            \]
            Evaluating at $(-20, 5, 1100)$, the instantaneous rate of change of the climber's altitude would be $-2\sqrt2\bp{-20 + 2\cdot5} = 20\sqrt2$ ft/s.

            \boxt{The climber would ascend at a rate of $20\sqrt2$ feet per second.}

        \part
            For a level path, the instantaneous rate of change of the climber's altitude should be 0. Let the direction of the climber be $u = \cvecii{a}{b}$. Consider $\evalder{D_{\vec u} f(x, y)}{(-20, 5)} = 0$.
            \begin{alignat*}{2}
                &&\evalder{D_{\vec u} f(x, y)}{(-20, 5)} &= 0\\
                \implies&& -4\cvecii{-20}{10} \cdot \cvecii{a}{b} &= 0\\
                \implies&&-2a + b &= 0\\
                \implies&&b &= 2a
            \end{alignat*}
            We hence have $\vec u = \cvecii{a}{b} = \cvecii{a}{2a} = a\cvecii12$.

            \boxt{The climber should walk in the direction of $\cvecii{1}{2}$.}

    \problem{}
        Find the absolute maximum and minimum values of $f(x, y) = 3xy - 6x - 3y + 7$ on the closed triangular region $R$ with vertices $(0, 0)$, $(3, 0)$ and $(0, 5)$.
    
    \solution
        Note that $f_x(x, y) = 3y - 6$ and $f_y(x, y) = 3x - 3$, whence $f_{xx}(x, y) = f_{yy}(x, y) = 0$ and $f_{xy} = 3$. For stationary points, $\nabla f = \vec 0 \implies \cvecii{3y-6}{3x-3} = \vec 0 \implies x = 1, y = 2$.

        Consider the nature of the stationary point at $(1, 2)$. We have \[D = f_{xx}(1, 2)f_{yy}(1, 2) - \bs{f_{xy}(1, 2)}^2 = -9 < 0\] Hence, by the second derivative test, we see that $f(x, y)$ has a saddle point at $(1, 2)$. Thus, the extrema of $f(x, y)$ must occur along its boundary.

        Note that the boundary of $f(x, y)$ is given by
        \begin{itemize}
            \item $x = 0$, $y \in [0, 5]$
            \item $x \in [0, 3]$, $y = 0$
            \item $x \in [0, 3]$, $y = 5 - \dfrac53 x$
        \end{itemize}

        \case{1}{$x = 0$, $y \in [0,5]$.} We have that $f(0, y) = -3y + 7$, which clearly attains a maximum of 7 at $y = 0$ and a minimum of $-8$ at $y = 5$.

        \case{2}{$x \in [0, 3]$, $y = 0$.} We have that $f(x, 0) = -6x + 7$, which clearly attains a maximum of 7 at $x = 0$ and a minimum of $-11$ at $x = 3$.

        \case{3}{$x \in [0, 3]$, $y = 5 - \dfrac53 x$.} Observe that
        \begin{align*}
            f\of{x, 5 - \dfrac53 x} &= 3x\bp{5 - \dfrac53 x} - 6x - 3\bp{5 - \dfrac53 x} + 7\\
            &= -5x^2 + 14x - 8\\
            &= -(x-2)(5x-4)
        \end{align*}
        is concave down and has a turning point at $x = 1.4$. Hence, the function clearly attains a maximum of $1.8$ when $x = 1.4$ and a minimum of $-11$ when $x = 3$ (note that at $x = 0$, the function returns $-8$). 

        Hence, the maximum of $f(x, y)$ is 7, while the minimum is $-11$.

        \boxt{$\max f(x, y) = 7$, $\min f(x, y) = -11$}

    \problem{}
        Find the dimensions of a rectangular box, open at the top, having a volume of 32 cm$^3$, and requiring the least amount of material for its construction.

    \solution
        Let the box have side lengths of $x$, $y$ and $z$ cm. Given that the volume of the box is fixed at 32 cm$^3$, we have \[xyz = 32 \implies z = \dfrac{32}{xy}\] Let the surface area of the box be measured by $f(x, y)$. Then
        \begin{align*}
            f(x, y) &= xy + 2yz + 2xz\\
            &= xy + 2y\bp{\dfrac{32}{xy}} + 2x\bp{\dfrac{32}{xy}}\\
            &= xy + 64x^{-1} + 64y^{-1}
        \end{align*}
        Note that $\nabla f = \cvecii{f_x(x, y)}{f_y(x, y)} = \cvecii{y-64x^{-2}}{x - 64y^{-2}}$. For stationary points, $\nabla f = \vec 0$. We hence obtain
        \[
            \begin{cases}
                y = 64x^{-2}\\
                x = 64y^{-2}
            \end{cases} \implies
            \begin{cases}
                yx^2 = 64\\
                xy^2 = 64
            \end{cases}
            \implies x^3y^3 = 64^2 \implies xy = 16
        \]
        Hence, $x = \dfrac{x^2y}{xy} = \dfrac{64}{16} = 4$, implying that $y = 4$ and $z = 2$. Hence, $f(x, y)$ has a stationary point at $(4, 4, 2)$. 
        
        We now consider the nature of this stationary point. Note that $f_{xx}(x, y) = 128x^{-3}$, $f_{yy} = 128y^{-3}$ and $f_{xy} = 1$. Hence, \[D = f_{xx}(4, 4)f_{yy}(4, 4) - \bs{f_{xy}(4, 4)}^2 = 3\] Since $D > 0$ and $f_{xx}(4, 4) = 2 > 0$, by the second derivative test, $f(x, y)$ attains a minimum at $(4, 4, 2)$. Thus, the amount of material required is lowest for a box of dimension $4 \times 4 \times 2$.

        \boxt{The dimensions of the box are 4 cm by 4 cm by 2 cm.}

    \problem{}
        Find the quadratic approximation of $f(x, y) = x^2 y + xy^2$ around the point $(1, 1)$.

    \solution
        Taking partial derivatives, we have
        \begin{align*}
            f_x(x, y) &= 2xy + y^2\\
            f_y(x, y) &= 2xy + x^2\\
            f_{xx}(x, y) &= 2y\\
            f_{xy}(x, y) &= 2x + 2y\\
            f_{yy}(x, y) &= 2x
        \end{align*}
        Hence, the required quadratic approximation $Q(x, y)$ is given by
        \begin{align*}
            Q(x, y) &= f(1, 1) + f_x(1, 1)(x-1) + f_y(1, 1)(y-1)\\
            & \hspace{3em} + \dfrac12 f_{xx}(1, 1)(x-1)^2 + f_{xy}(1, 1)(x-1)(y-1) + \dfrac12 f_{yy}(1, 1)(y-1)^2\\
            &= 2 + 3(x - 1) + 3(y - 1) + (x-1)^2 + 4(x-1)(y-1) + (y-1)^2\\
            &= 2 + (3x-3) + (3y-3) + (x^2 - 2x + 1) + (4xy - 4x - 4y + 4) + (y^2 - 2y + 1)\\
            &= 2 - 3x - 3y + 4xy + x^2 + y^2
        \end{align*}

        \boxt{$Q(x, y) = 2 - 3x - 3y + 4xy + x^2 + y^2$}

\end{document}